$$\dfrac{d}{dx} \sigma(x) &= \dfrac{d}{dx} \left[ \dfrac{1}{1 + e^{-x}} \right] \\
&= \dfrac{d}{dx} \left( 1 + \mathrm{e}^{-x} \right)^{-1} \\
&= -(1 + e^{-x})^{-2}(-e^{-x}) \\
&= \dfrac{e^{-x}}{\left(1 + e^{-x}\right)^2} \\
&= \dfrac{1}{1 + e^{-x}\ } \cdot \dfrac{e^{-x}}{1 + e^{-x}}  \\
&= \dfrac{1}{1 + e^{-x}\ } \cdot \dfrac{(1 + e^{-x}) - 1}{1 + e^{-x}}  \\
&= \dfrac{1}{1 + e^{-x}\ } \cdot \left( \dfrac{1 + e^{-x}}{1 + e^{-x}} - \dfrac{1}{1 + e^{-x}} \right) \\
&= \dfrac{1}{1 + e^{-x}\ } \cdot \left( 1 - \dfrac{1}{1 + e^{-x}} \right) \\
&= \sigma(x) \cdot (1 - \sigma(x))$$
